Stlc/Lec3.v
@@ -12,90 +12,7 @@ Require Import Stlc.Definitions.
 (** And some auxiliary lemmas about these definitions. *)
 Require Import Stlc.Lemmas.
 
-Require Import Stlc.Lec2.
-
-(*************************************************************)
-
-Inductive res (a : Set) : Set :=
-  | val     : a -> res a
-  | timeout : res a
-  | stuck   : res a.
-
-Fixpoint n_bigstep (n:nat) (e:exp) : res exp :=
-  match n with
-  | 0 => @timeout exp
-  | S m =>
-    match e with
-    | var_b n => @stuck exp
-    | var_f x => @stuck exp
-    | app e1 e2 =>
-      match n_bigstep m e1 with
-      | val _ (abs T e1') =>
-        match n_bigstep m e2 with
-        | val _ v1 =>
-          n_bigstep m (open e1' v1)
-        | r => r
-        end
-      | r       => r
-      end
-    | abs T e   => val _ (abs T e)
-    end
-  end.
-
-(* Type soundness for the definitional interpreter.
-   If the interpreter doesn't timeout, then it doesn't get stuck. *)
-
-Lemma n_bigstep_eval : forall n e T,
-  typing nil e T ->
-  @timeout exp <> n_bigstep n e ->
-  exists v, val _ v = n_bigstep n e /\ typing nil v T /\ is_value_of_exp v.
-Proof.
-  induction n; intros e T TE EV; simpl in *.
-  contradiction.
-  destruct e; inversion TE; subst.
-  - Case "var_f". inversion H2.
-  - Case "abs".
-    exists (abs T0 e). split; simpl; eauto.
-  - Case "app".
-    pose (Ih1 := IHn e1 (typ_arrow T1 T) H2). clearbody Ih1.
-    pose (Ih2 := IHn e2 T1 H4). clearbody Ih2.
-
-    destruct (n_bigstep n e1); try contradiction;
-    destruct Ih1 as [v1 [EV1 [Tv1 vv1]]];
-       try solve [intro h; inversion h]; inversion EV1.
-
-    (* By canonical forms, know that v1 must be an abstraction. *)
-    destruct v1; simpl in vv1; try contradiction; clear vv1. subst e.
-
-    destruct (n_bigstep n e2); try contradiction;
-    destruct Ih2 as [v2 [EV2 [Tv2 vv2]]];
-        try solve [intro h; inversion h]; inversion EV2. subst.
-
-    eapply IHn; eauto.
-
-    (* result typechecks *)
-    inversion Tv1. subst.
-    pick fresh x.
-    rewrite (subst_exp_intro x).
-    eapply typing_subst_simple; eauto.
-    fsetdec.
-Qed.
-
-(*************************************************************)
-
-Inductive bigstep : exp -> exp -> Prop :=    (* defn bigstep *)
- | bs_app : forall (e1 v2:exp) (T1:typ) (e1' e2 v1:exp),
-     is_value_of_exp v1 ->
-     bigstep e1 (abs T1 e1') ->
-     bigstep e2 v1 ->
-     bigstep  (open_exp_wrt_exp  e1' v1 )  v2 ->
-     bigstep (app e1 e2) v2
-| bs_val : forall (v:exp),
-     is_value_of_exp v ->
-     lc_exp v ->
-     bigstep v v.
-Hint Constructors bigstep.
-
+(* This file draws heavily on the generated lemmas in Stlc.Lemmas. *)
 
 (*************************************************************)
 (*   Connection to nominal representation of terms           *)
@@ -142,6 +59,11 @@ Fixpoint rho_lookup x rho : option nom_val :=
   | nom_nil => None
   | nom_cons y v rho' =>  if (x == y) then Some v else rho_lookup x rho'
   end.
+
+Inductive res (a : Set) : Set :=
+  | val     : a -> res a
+  | timeout : res a
+  | stuck   : res a.
 
 Fixpoint nom_interp (n:nat) (e:n_exp) (rho: nom_env) : res nom_val :=
   match n with
@@ -199,8 +121,6 @@ end.
    nominal terms.
  *)
 
-Notation "[ z ~> u ] e" := (subst_exp u z e) (at level 68).
-
 Fixpoint nom_val_to_exp (cv:nom_val) : exp :=
   match cv with
   | nom_closure x T rho e =>
@@ -213,9 +133,10 @@ with nom_envsubst (ne:nom_env) : exp -> exp :=
   end.
 
 
+(* ----------------- closed values, environments and terms ------------------- *)
 
 (*
-    However, to prove the soundness lemma, we will need to strengthen it so
+    To prove the soundness lemma, we will need to strengthen it so
     that it says something about non-empty environments.
 
 
@@ -227,9 +148,10 @@ with nom_envsubst (ne:nom_env) : exp -> exp :=
 >>
 
    However, this lemma will not be true for all environments and nominal terms,
-   we need to make sure that the domain of the environment includes definitions
-   for all of the free variables in e, and that the range of the environment
-   includes only *closed* nominal values.
+   we need to make sure that
+     (1) the domain of the environment includes definitions for all
+         of the free variables in e, and
+     (2) the range of the environment includes only *closed* nominal values.
 
 *)
 
@@ -239,10 +161,11 @@ Fixpoint dom_rho (rho :nom_env) :=
   | nom_cons x v rho => {{x}} \u dom_rho rho
   end.
 
+
 Inductive closed_val : nom_val -> Prop :=
   | closed_closure : forall x T rho e,
       closed_env rho ->
-      fv_exp (nom_to_exp e) [<=] {{x}} \u dom_rho rho ->
+      fv_exp (nom_to_exp e) [<=] add x (dom_rho rho) ->
       closed_val (nom_closure x T rho e)
 with closed_env : nom_env -> Prop :=
      | closed_nil : closed_env nom_nil
@@ -250,10 +173,35 @@ with closed_env : nom_env -> Prop :=
          closed_val v -> closed_env rho -> closed_env (nom_cons x v rho).
 Hint Constructors closed_env closed_val.
 
+(* Our definition of closed_env means that any value that we lookup
+   from this environment will be closed. *)
+
+Lemma rho_lookup_closed_val : forall x rho v,
+    closed_env rho ->
+    Some v = rho_lookup x rho ->
+    closed_val v.
+Proof.
+  induction rho; intros; simpl in *.
+  - inversion H0.
+  - inversion H. subst.
+    destruct (x == a).
+    inversion H0. eauto.
+    eapply IHrho; eauto.
+Qed.
+
+(* Furthermore, we can also prove that closed values have no
+   free variables after translation.
+
+   This proof is done by mutual induction on the closed_val/closed_env
+   derivation. So before we can do that, we need to ask Coq to
+   derive the appropriate induction scheme.
+*)
+
 
 Scheme closed_val_ind' := Induction for closed_val Sort Prop
  with  closed_env_ind' := Induction for closed_env Sort Prop.
 Combined Scheme closed_nom from closed_val_ind', closed_env_ind'.
+
 
 Lemma fv_closed_mutual :
   (forall v, closed_val v -> fv_exp (nom_val_to_exp v) [=] {}) /\
@@ -262,7 +210,8 @@ Lemma fv_closed_mutual :
 Proof.
   eapply closed_nom; intros.
   + simpl. rewrite H. fsetdec.
-    simpl. autorewrite with lngen.
+    simpl.
+    rewrite fv_exp_close_exp_wrt_exp.
     fsetdec.
   + simpl in *. fsetdec.
   + simpl in *.
@@ -285,132 +234,10 @@ Proof.
   eapply fv_closed_mutual.
 Qed.
 
+(* Now we can use these results to show that the interpreter
+   produces closed values from appropriate environments and terms. *)
 
-(*
-Fixpoint nom_fv (e : n_exp) : vars :=
-  match e with
-  | n_var x => {{ x }}
-  | n_abs x T e => AtomSetImpl.remove x (nom_fv e)
-  | n_app e1 e2 => nom_fv e1 \u nom_fv e2
-  end.
-
-Lemma nom_to_exp_fv : forall ne, nom_fv ne [=] fv_exp (nom_to_exp ne).
-Proof.
-  induction ne; simpl in *.
-  - fsetdec.
-  - rewrite IHne.
-    autorewrite with lngen.
-    fsetdec.
-  - rewrite IHne1. rewrite IHne2.
-    fsetdec.
-Qed.
-
-*)
-
-Lemma nom_to_exp_lc : forall ne, lc_exp (nom_to_exp ne).
-Proof.
-  induction ne; simpl; auto.
-  eapply lc_abs_exists with (x := x).
-  rewrite open_exp_wrt_exp_close_exp_wrt_exp.
-  auto.
-Qed.
-
-Scheme nom_val_ind' := Induction for nom_val Sort Prop
- with  nom_env_ind' := Induction for nom_env Sort Prop.
-Combined Scheme nom_mutual from nom_val_ind', nom_env_ind'.
-
-
-
-Lemma unload_fresh : forall rho v,
-    closed_val v ->
-    nom_envsubst rho (nom_val_to_exp v) = nom_val_to_exp v.
-Proof.
-  induction rho. simpl. auto.
-  intros. simpl.
-  rewrite subst_exp_fresh_eq; auto.
-  rewrite fv_closed; auto.
-Qed.
-
-
-Lemma rho_lookup_closed_val : forall x rho v,
-    closed_env rho ->
-    Some v = rho_lookup x rho ->
-    closed_val v.
-Proof.
-  induction rho; intros; simpl in *.
-  - inversion H0.
-  - inversion H. subst.
-    destruct (x == a).
-    default_simp.
-    eapply IHrho; eauto.
-Qed.
-
-Lemma nom_envsubst_var : forall x rho v,
-    closed_env rho ->
-    Some v = rho_lookup x rho ->
-    nom_envsubst rho (var_f x) = nom_val_to_exp v.
-Proof.
-  induction rho.
-  - intros. simpl in *.
-  inversion H0.
-  -  intros. simpl in *.
-     inversion H. subst.
-     destruct (x == a).
-     + inversion H0. subst. clear H0.
-    simpl.
-    rewrite unload_fresh; auto.
-  + eapply IHrho; auto.
-Qed.
-
-Lemma nom_envsubst_abs : forall rho T e,
- nom_envsubst rho (abs T e) = abs T (nom_envsubst rho e).
-Proof.
-  induction rho; simpl.
-  - auto.
-  - intros.
-    rewrite IHrho.
-    auto.
-Qed.
-
-Lemma nom_envsubst_app : forall rho e1 e2,
- nom_envsubst rho (app e1 e2) = app (nom_envsubst rho e1) (nom_envsubst rho e2).
-Proof.
-  induction rho; simpl.
-  - auto.
-  - intros.
-    rewrite IHrho.
-    auto.
-Qed.
-
-Lemma nom_val_to_exp_is_value : forall v, is_value_of_exp (nom_val_to_exp v).
-Proof.
-  destruct v. simpl. rewrite nom_envsubst_abs.
-  simpl. auto.
-Qed.
-
-Lemma nom_val_to_exp_lc_mutual :
-  (forall v, lc_exp (nom_val_to_exp v)) /\
-  (forall rho, forall e, lc_exp e -> lc_exp (nom_envsubst rho e)).
-Proof.
-  eapply nom_mutual.
-  - intros. simpl.
-    eapply H.
-    eapply lc_abs_exists with (x:=a).
-    autorewrite with lngen.
-    eapply nom_to_exp_lc.
-  - intros. simpl. auto.
-  - intros; simpl in *.
-    eapply H0; eauto.
-    eapply subst_exp_lc_exp; eauto.
-Qed.
-
-Lemma nom_envsubst_lc : (forall rho, forall e, lc_exp e -> lc_exp (nom_envsubst rho e)).
-  eapply nom_val_to_exp_lc_mutual.
-Qed.
-
-
-
-Lemma nom_closed : forall n rho e v,
+Lemma nom_interp_closed : forall n rho e v,
     val _ v = nom_interp n e rho ->
     closed_env rho ->
     fv_exp (nom_to_exp e) [<=] dom_rho rho ->
@@ -424,58 +251,164 @@ Proof.
     destruct (rho_lookup x rho);
     inversion H;  auto.
   - Case "abs".
-    inversion H.
+    inversion H.  subst.
     econstructor; eauto.
-    autorewrite with lngen in H1.
+    rewrite fv_exp_close_exp_wrt_exp in H1.
     rewrite <- H1.
-    rewrite <-  AtomSetProperties.add_union_singleton.
+    (* TODO: see why fsetdec cannot do this. *)
     eapply FSetDecideTestCases.test_Subset_add_remove.
+
   - Case "app".
     remember (nom_interp n e1 rho) as r1.
     remember (nom_interp n e2 rho) as r2.
     destruct r1; try solve [inversion H].
-
-    assert (C: closed_val n0). eapply IHn; eauto. fsetdec.
+    assert (C1: closed_val n0). eapply IHn; eauto. fsetdec.
     destruct n0 as [x T rho' e1'].
-    inversion C.
+    inversion C1. simpl in H7.
+
     destruct r2; try solve [inversion H].
-    assert (closed_val n0). eapply IHn; eauto. fsetdec.
-    eauto.
+    assert (C2: closed_val n0). eapply IHn; eauto. fsetdec.
+
+    subst.
+    eapply IHn; eauto.
+    simpl.
+    fsetdec.
 Qed.
 
+(* ----------------- nom_envsubst reductions ------------------- *)
+
+(* We can think of a an environment as a multi-substitution for locally
+   nameless terms.
+
+   Therefore, the nom_envsubst function inherits many of the properties of the
+   subst_exp function.
+
+ *)
 
 
-
-Lemma commute_subst_envsubst : forall rho x v e,
-  closed_env rho ->
-  closed_val v  ->
-  x \notin dom_rho rho ->
-  nom_envsubst rho ([x ~> nom_val_to_exp v] e) =
-                    [x ~> nom_val_to_exp v] nom_envsubst rho e.
+Lemma nom_envsubst_fresh_eq : forall rho v,
+    closed_val v ->
+    nom_envsubst rho (nom_val_to_exp v) = nom_val_to_exp v.
 Proof.
-  induction rho.
-  - intros. simpl. auto.
-  - intros.
-    simpl in *.
-    inversion H.
-    rewrite subst_exp_subst_exp; auto.
-    rewrite (subst_exp_fresh_eq (nom_val_to_exp v)); auto.
-    rewrite fv_closed; auto.
-    rewrite fv_closed; auto.
+  induction rho. simpl. auto.
+  intros. simpl.
+  rewrite subst_exp_fresh_eq; auto.
+  rewrite fv_closed; auto.
 Qed.
 
-Lemma open_nom_envsubst : forall rho e e',
- fv_exp e' [=] {} ->
- (open_exp_wrt_exp (nom_envsubst rho e) e') =
- nom_envsubst rho (open_exp_wrt_exp e e').
+Lemma nom_envsubst_open : forall rho e e',
+ (forall v, lc_exp (nom_val_to_exp v)) ->
+ (nom_envsubst rho (open e e')) = (open (nom_envsubst rho e) (nom_envsubst rho e')).
 Proof.
   induction rho; intros; simpl. auto.
-  rewrite subst_exp_open_exp_wrt_exp.
-  rewrite (subst_exp_fresh_eq e'); auto.
-  rewrite H.
-  fsetdec.
+  rewrite subst_exp_open_exp_wrt_exp; eauto.
+Qed.
+
+
+Lemma nom_envsubst_var : forall x rho v,
+    closed_env rho ->
+    Some v = rho_lookup x rho ->
+    nom_envsubst rho (var_f x) = nom_val_to_exp v.
+Proof.
+  induction rho.
+  - intros. simpl in *. inversion H0.
+  - intros. simpl in *.
+     inversion H. subst.
+     destruct (x == a).
+     + inversion H0. subst. clear H0.
+    simpl.
+    rewrite nom_envsubst_fresh_eq; auto.
+  + eapply IHrho; auto.
+Qed.
+
+Lemma nom_envsubst_abs : forall rho T e,
+ nom_envsubst rho (abs T e) = abs T (nom_envsubst rho e).
+Proof.
+  induction rho; simpl; eauto.
+Qed.
+
+Lemma nom_envsubst_app : forall rho e1 e2,
+ nom_envsubst rho (app e1 e2) = app (nom_envsubst rho e1) (nom_envsubst rho e2).
+Proof.
+  induction rho; simpl; eauto.
+Qed.
+
+
+(* ----------------- interpreter soundness for values ------------------- *)
+
+(* The next step is to show that nominal values bigstep to themselves.
+   In otherwords, we want to show that:
+
+<<
+   Lemma nom_soundness_val : forall v,
+       bigstep (nom_val_to_exp v) (nom_val_to_exp v).
+>>
+
+  To prove this lemma, we need to show that these nominal values translate
+  LN values, and that these values are locally closed.
+
+*)
+
+Lemma nom_val_to_exp_is_value : forall v, is_value_of_exp (nom_val_to_exp v).
+Proof.
+  destruct v. simpl. rewrite nom_envsubst_abs.
+  simpl. auto.
+Qed.
+
+Hint Resolve nom_val_to_exp_is_value.
+
+Lemma nom_to_exp_lc : forall ne, lc_exp (nom_to_exp ne).
+Proof.
+  induction ne; simpl; auto.
+  eapply lc_abs_exists with (x1 := x).
+  rewrite open_exp_wrt_exp_close_exp_wrt_exp.
+  auto.
+Qed.
+
+
+(* Need the mutual induction scheme for the next lemma! *)
+Scheme nom_val_ind' := Induction for nom_val Sort Prop
+ with  nom_env_ind' := Induction for nom_env Sort Prop.
+Combined Scheme nom_mutual from nom_val_ind', nom_env_ind'.
+
+
+Lemma nom_val_to_exp_lc_mutual :
+  (forall v, lc_exp (nom_val_to_exp v)) /\
+  (forall rho, forall e, lc_exp e -> lc_exp (nom_envsubst rho e)).
+Proof.
+  eapply nom_mutual.
+  - intros. simpl.
+    eapply H.
+    eapply lc_abs_exists with (x1:=a).
+    rewrite open_exp_wrt_exp_close_exp_wrt_exp.
+    eapply nom_to_exp_lc.
+  - intros. simpl. auto.
+  - intros; simpl in *.
+    eapply H0; eauto.
+    eapply subst_exp_lc_exp; eauto.
+Qed.
+
+Lemma nom_val_to_exp_lc : forall v,
+    lc_exp (nom_val_to_exp v).
+Proof.
   eapply nom_val_to_exp_lc_mutual.
 Qed.
+Lemma nom_envsubst_lc : (forall rho, forall e, lc_exp e -> lc_exp (nom_envsubst rho e)).
+  eapply nom_val_to_exp_lc_mutual.
+Qed.
+
+Hint Resolve nom_to_exp_lc nom_val_to_exp_lc nom_envsubst_lc.
+
+Lemma nom_soundness_val : forall v,
+       bigstep (nom_val_to_exp v) (nom_val_to_exp v).
+Proof.
+  eauto.
+Qed.
+
+(* ----------------- interpreter soundness ------------------- *)
+
+(* Finally, we get to the actual soundness function for the interpreter. *)
+
 
 Lemma nom_soundness : forall n rho e v,
     val _ v = nom_interp n e rho  ->
@@ -488,53 +421,39 @@ Proof.
   intros.  destruct e; simpl in *.
   - Case "var".
     remember (rho_lookup x rho) as l.
-    destruct l as [[w Pr]| Pr].
-    inversion H. subst. clear H1.
+    destruct l; inversion H.
     erewrite nom_envsubst_var; eauto.
-    econstructor; eauto.
-    eapply nom_val_to_exp_is_value.
-    eapply nom_val_to_exp_lc_mutual.
-    eapply nom_to_exp_lc.
-    inversion H.
   - Case "abs".
     inversion H.
-    subst.
-    simpl.
-    rewrite nom_envsubst_abs.
-    econstructor; eauto.
-    simpl. auto.
-    rewrite <- nom_envsubst_abs.
-    eapply nom_envsubst_lc.
-    eapply lc_abs_exists with (x := x).
-    autorewrite with lngen.
-    eapply nom_to_exp_lc.
+    replace (nom_envsubst rho (abs T (close_exp_wrt_exp x (nom_to_exp e)))) with
+            (nom_val_to_exp (nom_closure x T rho e)); auto.
   - Case "app".
     remember (nom_interp n e1 rho) as r1.
     remember (nom_interp n e2 rho) as r2.
     destruct r1; try solve [inversion H].
-    assert (closed_val n0). eapply nom_closed; eauto. fsetdec.
-    destruct n0 as [x T rho' e1'].
-    inversion H2.
-    destruct r2; try solve [inversion H].
-    assert (closed_val n0).
-    eapply nom_closed; eauto. fsetdec.
-
+    destruct (nom_interp_closed _ _ _ _ Heqr1); eauto; try fsetdec.
     apply IHn in Heqr1; auto; try fsetdec.
+
+    destruct r2; try solve [inversion H].
+    destruct (nom_interp_closed _ _ _ _ Heqr2); eauto; try fsetdec.
     apply IHn in Heqr2; auto; try fsetdec.
+
     simpl in Heqr1.
     rewrite nom_envsubst_abs in Heqr1.
 
-    apply IHn in H; eauto.
+    apply IHn in H; eauto; simpl; try fsetdec.
     simpl in H.
 
+    rewrite subst_exp_spec in H.
+    rewrite nom_envsubst_open in H; eauto.
+
+    replace (nom_envsubst rho1 (abs T0 (close_exp_wrt_exp x0 (nom_to_exp e0)))) with
+            (nom_val_to_exp (nom_closure x0 T0 rho1 e0)) in H; auto.
+
+    rewrite nom_envsubst_fresh_eq in H; eauto.
+
     rewrite nom_envsubst_app.
-    econstructor; eauto.
-    apply nom_val_to_exp_is_value.
-    rewrite open_nom_envsubst.
-    rewrite <- subst_exp_spec.
-    auto.
-    rewrite fv_closed. fsetdec.
-    auto.
+    eauto.
 Qed.
 
 Lemma completeness : forall e v rho,
@@ -542,30 +461,3 @@ Lemma completeness : forall e v rho,
     exists n, nom_interp n e rho = val _ v.
 Proof.
 Admitted.
-
-(*
-Definition fmap_res {a b : Set} (f : a -> b) (r : res a) : res b :=
-  match r with
-  | val _ v => val _ (f v)
-  | timeout _ => timeout _
-  | stuck   _ => stuck   _
-  end.
-
-Lemma n_nom_soundness : forall n rho e r,
-    r = nom_interp n e rho  ->
-    closed_env rho ->
-    nom_fv e [<=] dom_rho rho ->
-    fmap_res nom_val_to_exp r = n_bigstep n (nom_envsubst rho (nom_to_exp e)).
-Proof.
-  induction n; intros. simpl in *. subst. simpl. auto.
-  destruct e. simpl in *.
-  - Case "var".
-    remember (rho_lookup x rho) as l.
-    destruct l.
-    erewrite nom_envsubst_var; eauto.
-    destruct n0 as [T y rho' e']. simpl.
-    rewrite nom_envsubst_abs. subst r. simpl.
-    rewrite nom_envsubst_abs. auto.
-    admit.
-  - Case "abs".
-*)
